Mathbin/Computability/Reduce.lean
@@ -35,6 +35,7 @@ universe u v w
 
 open Function
 
+#print ManyOneReducible /-
 /--
 `p` is many-one reducible to `q` if there is a computable function translating questions about `p`
 to questions about `q`.
@@ -42,20 +43,35 @@ to questions about `q`.
 def ManyOneReducible {α β} [Primcodable α] [Primcodable β] (p : α → Prop) (q : β → Prop) :=
   ∃ f, Computable f ∧ ∀ a, p a ↔ q (f a)
 #align many_one_reducible ManyOneReducible
+-/
 
 -- mathport name: «expr ≤₀ »
 infixl:1000 " ≤₀ " => ManyOneReducible
 
+/- warning: many_one_reducible.mk -> ManyOneReducible.mk is a dubious translation:
+lean 3 declaration is
+  forall {α : Type.{u1}} {β : Type.{u2}} [_inst_1 : Primcodable.{u1} α] [_inst_2 : Primcodable.{u2} β] {f : α -> β} (q : β -> Prop), (Computable.{u1, u2} α β _inst_1 _inst_2 f) -> (ManyOneReducible.{u1, u2} α β _inst_1 _inst_2 (fun (a : α) => q (f a)) q)
+but is expected to have type
+  forall {α : Type.{u2}} {β : Type.{u1}} [_inst_1 : Primcodable.{u2} α] [_inst_2 : Primcodable.{u1} β] {f : α -> β} (q : β -> Prop), (Computable.{u2, u1} α β _inst_1 _inst_2 f) -> (ManyOneReducible.{u2, u1} α β _inst_1 _inst_2 (fun (a : α) => q (f a)) q)
+Case conversion may be inaccurate. Consider using '#align many_one_reducible.mk ManyOneReducible.mkₓ'. -/
 theorem ManyOneReducible.mk {α β} [Primcodable α] [Primcodable β] {f : α → β} (q : β → Prop)
     (h : Computable f) : (fun a => q (f a)) ≤₀ q :=
   ⟨f, h, fun a => Iff.rfl⟩
 #align many_one_reducible.mk ManyOneReducible.mk
 
+#print manyOneReducible_refl /-
 @[refl]
 theorem manyOneReducible_refl {α} [Primcodable α] (p : α → Prop) : p ≤₀ p :=
   ⟨id, Computable.id, by simp⟩
 #align many_one_reducible_refl manyOneReducible_refl
+-/
 
+/- warning: many_one_reducible.trans -> ManyOneReducible.trans is a dubious translation:
+lean 3 declaration is
+  forall {α : Type.{u1}} {β : Type.{u2}} {γ : Type.{u3}} [_inst_1 : Primcodable.{u1} α] [_inst_2 : Primcodable.{u2} β] [_inst_3 : Primcodable.{u3} γ] {p : α -> Prop} {q : β -> Prop} {r : γ -> Prop}, (ManyOneReducible.{u1, u2} α β _inst_1 _inst_2 p q) -> (ManyOneReducible.{u2, u3} β γ _inst_2 _inst_3 q r) -> (ManyOneReducible.{u1, u3} α γ _inst_1 _inst_3 p r)
+but is expected to have type
+  forall {α : Type.{u3}} {β : Type.{u2}} {γ : Type.{u1}} [_inst_1 : Primcodable.{u3} α] [_inst_2 : Primcodable.{u2} β] [_inst_3 : Primcodable.{u1} γ] {p : α -> Prop} {q : β -> Prop} {r : γ -> Prop}, (ManyOneReducible.{u3, u2} α β _inst_1 _inst_2 p q) -> (ManyOneReducible.{u2, u1} β γ _inst_2 _inst_3 q r) -> (ManyOneReducible.{u3, u1} α γ _inst_1 _inst_3 p r)
+Case conversion may be inaccurate. Consider using '#align many_one_reducible.trans ManyOneReducible.transₓ'. -/
 @[trans]
 theorem ManyOneReducible.trans {α β γ} [Primcodable α] [Primcodable β] [Primcodable γ]
     {p : α → Prop} {q : β → Prop} {r : γ → Prop} : p ≤₀ q → q ≤₀ r → p ≤₀ r
@@ -63,14 +79,19 @@ theorem ManyOneReducible.trans {α β γ} [Primcodable α] [Primcodable β] [Pri
     ⟨g ∘ f, c₂.comp c₁, fun a => ⟨fun h => by rwa [← h₂, ← h₁], fun h => by rwa [h₁, h₂]⟩⟩
 #align many_one_reducible.trans ManyOneReducible.trans
 
+#print reflexive_manyOneReducible /-
 theorem reflexive_manyOneReducible {α} [Primcodable α] : Reflexive (@ManyOneReducible α α _ _) :=
   manyOneReducible_refl
 #align reflexive_many_one_reducible reflexive_manyOneReducible
+-/
 
+#print transitive_manyOneReducible /-
 theorem transitive_manyOneReducible {α} [Primcodable α] : Transitive (@ManyOneReducible α α _ _) :=
   fun p q r => ManyOneReducible.trans
 #align transitive_many_one_reducible transitive_manyOneReducible
+-/
 
+#print OneOneReducible /-
 /--
 `p` is one-one reducible to `q` if there is an injective computable function translating questions
 about `p` to questions about `q`.
@@ -78,20 +99,35 @@ about `p` to questions about `q`.
 def OneOneReducible {α β} [Primcodable α] [Primcodable β] (p : α → Prop) (q : β → Prop) :=
   ∃ f, Computable f ∧ Injective f ∧ ∀ a, p a ↔ q (f a)
 #align one_one_reducible OneOneReducible
+-/
 
 -- mathport name: «expr ≤₁ »
 infixl:1000 " ≤₁ " => OneOneReducible
 
+/- warning: one_one_reducible.mk -> OneOneReducible.mk is a dubious translation:
+lean 3 declaration is
+  forall {α : Type.{u1}} {β : Type.{u2}} [_inst_1 : Primcodable.{u1} α] [_inst_2 : Primcodable.{u2} β] {f : α -> β} (q : β -> Prop), (Computable.{u1, u2} α β _inst_1 _inst_2 f) -> (Function.Injective.{succ u1, succ u2} α β f) -> (OneOneReducible.{u1, u2} α β _inst_1 _inst_2 (fun (a : α) => q (f a)) q)
+but is expected to have type
+  forall {α : Type.{u2}} {β : Type.{u1}} [_inst_1 : Primcodable.{u2} α] [_inst_2 : Primcodable.{u1} β] {f : α -> β} (q : β -> Prop), (Computable.{u2, u1} α β _inst_1 _inst_2 f) -> (Function.Injective.{succ u2, succ u1} α β f) -> (OneOneReducible.{u2, u1} α β _inst_1 _inst_2 (fun (a : α) => q (f a)) q)
+Case conversion may be inaccurate. Consider using '#align one_one_reducible.mk OneOneReducible.mkₓ'. -/
 theorem OneOneReducible.mk {α β} [Primcodable α] [Primcodable β] {f : α → β} (q : β → Prop)
     (h : Computable f) (i : Injective f) : (fun a => q (f a)) ≤₁ q :=
   ⟨f, h, i, fun a => Iff.rfl⟩
 #align one_one_reducible.mk OneOneReducible.mk
 
+#print oneOneReducible_refl /-
 @[refl]
 theorem oneOneReducible_refl {α} [Primcodable α] (p : α → Prop) : p ≤₁ p :=
   ⟨id, Computable.id, injective_id, by simp⟩
 #align one_one_reducible_refl oneOneReducible_refl
+-/
 
+/- warning: one_one_reducible.trans -> OneOneReducible.trans is a dubious translation:
+lean 3 declaration is
+  forall {α : Type.{u1}} {β : Type.{u2}} {γ : Type.{u3}} [_inst_1 : Primcodable.{u1} α] [_inst_2 : Primcodable.{u2} β] [_inst_3 : Primcodable.{u3} γ] {p : α -> Prop} {q : β -> Prop} {r : γ -> Prop}, (OneOneReducible.{u1, u2} α β _inst_1 _inst_2 p q) -> (OneOneReducible.{u2, u3} β γ _inst_2 _inst_3 q r) -> (OneOneReducible.{u1, u3} α γ _inst_1 _inst_3 p r)
+but is expected to have type
+  forall {α : Type.{u3}} {β : Type.{u2}} {γ : Type.{u1}} [_inst_1 : Primcodable.{u3} α] [_inst_2 : Primcodable.{u2} β] [_inst_3 : Primcodable.{u1} γ] {p : α -> Prop} {q : β -> Prop} {r : γ -> Prop}, (OneOneReducible.{u3, u2} α β _inst_1 _inst_2 p q) -> (OneOneReducible.{u2, u1} β γ _inst_2 _inst_3 q r) -> (OneOneReducible.{u3, u1} α γ _inst_1 _inst_3 p r)
+Case conversion may be inaccurate. Consider using '#align one_one_reducible.trans OneOneReducible.transₓ'. -/
 @[trans]
 theorem OneOneReducible.trans {α β γ} [Primcodable α] [Primcodable β] [Primcodable γ] {p : α → Prop}
     {q : β → Prop} {r : γ → Prop} : p ≤₁ q → q ≤₁ r → p ≤₁ r
@@ -100,28 +136,50 @@ theorem OneOneReducible.trans {α β γ} [Primcodable α] [Primcodable β] [Prim
       ⟨fun h => by rwa [← h₂, ← h₁], fun h => by rwa [h₁, h₂]⟩⟩
 #align one_one_reducible.trans OneOneReducible.trans
 
+/- warning: one_one_reducible.to_many_one -> OneOneReducible.to_many_one is a dubious translation:
+lean 3 declaration is
+  forall {α : Type.{u1}} {β : Type.{u2}} [_inst_1 : Primcodable.{u1} α] [_inst_2 : Primcodable.{u2} β] {p : α -> Prop} {q : β -> Prop}, (OneOneReducible.{u1, u2} α β _inst_1 _inst_2 p q) -> (ManyOneReducible.{u1, u2} α β _inst_1 _inst_2 p q)
+but is expected to have type
+  forall {α : Type.{u2}} {β : Type.{u1}} [_inst_1 : Primcodable.{u2} α] [_inst_2 : Primcodable.{u1} β] {p : α -> Prop} {q : β -> Prop}, (OneOneReducible.{u2, u1} α β _inst_1 _inst_2 p q) -> (ManyOneReducible.{u2, u1} α β _inst_1 _inst_2 p q)
+Case conversion may be inaccurate. Consider using '#align one_one_reducible.to_many_one OneOneReducible.to_many_oneₓ'. -/
 theorem OneOneReducible.to_many_one {α β} [Primcodable α] [Primcodable β] {p : α → Prop}
     {q : β → Prop} : p ≤₁ q → p ≤₀ q
   | ⟨f, c, i, h⟩ => ⟨f, c, h⟩
 #align one_one_reducible.to_many_one OneOneReducible.to_many_one
 
+/- warning: one_one_reducible.of_equiv -> OneOneReducible.of_equiv is a dubious translation:
+lean 3 declaration is
+  forall {α : Type.{u1}} {β : Type.{u2}} [_inst_1 : Primcodable.{u1} α] [_inst_2 : Primcodable.{u2} β] {e : Equiv.{succ u1, succ u2} α β} (q : β -> Prop), (Computable.{u1, u2} α β _inst_1 _inst_2 (coeFn.{max 1 (max (succ u1) (succ u2)) (succ u2) (succ u1), max (succ u1) (succ u2)} (Equiv.{succ u1, succ u2} α β) (fun (_x : Equiv.{succ u1, succ u2} α β) => α -> β) (Equiv.hasCoeToFun.{succ u1, succ u2} α β) e)) -> (OneOneReducible.{u1, u2} α β _inst_1 _inst_2 (Function.comp.{succ u1, succ u2, 1} α β Prop q (coeFn.{max 1 (max (succ u1) (succ u2)) (succ u2) (succ u1), max (succ u1) (succ u2)} (Equiv.{succ u1, succ u2} α β) (fun (_x : Equiv.{succ u1, succ u2} α β) => α -> β) (Equiv.hasCoeToFun.{succ u1, succ u2} α β) e)) q)
+but is expected to have type
+  forall {α : Type.{u2}} {β : Type.{u1}} [_inst_1 : Primcodable.{u2} α] [_inst_2 : Primcodable.{u1} β] {e : Equiv.{succ u2, succ u1} α β} (q : β -> Prop), (Computable.{u2, u1} α β _inst_1 _inst_2 (FunLike.coe.{max (succ u2) (succ u1), succ u2, succ u1} (Equiv.{succ u2, succ u1} α β) α (fun (_x : α) => (fun (x._@.Mathlib.Logic.Equiv.Defs._hyg.808 : α) => β) _x) (Equiv.instFunLikeEquiv.{succ u2, succ u1} α β) e)) -> (OneOneReducible.{u2, u1} α β _inst_1 _inst_2 (Function.comp.{succ u2, succ u1, 1} α β Prop q (FunLike.coe.{max (succ u2) (succ u1), succ u2, succ u1} (Equiv.{succ u2, succ u1} α β) α (fun (_x : α) => (fun (x._@.Mathlib.Logic.Equiv.Defs._hyg.808 : α) => β) _x) (Equiv.instFunLikeEquiv.{succ u2, succ u1} α β) e)) q)
+Case conversion may be inaccurate. Consider using '#align one_one_reducible.of_equiv OneOneReducible.of_equivₓ'. -/
 theorem OneOneReducible.of_equiv {α β} [Primcodable α] [Primcodable β] {e : α ≃ β} (q : β → Prop)
     (h : Computable e) : (q ∘ e) ≤₁ q :=
   OneOneReducible.mk _ h e.Injective
 #align one_one_reducible.of_equiv OneOneReducible.of_equiv
 
+/- warning: one_one_reducible.of_equiv_symm -> OneOneReducible.of_equiv_symm is a dubious translation:
+lean 3 declaration is
+  forall {α : Type.{u1}} {β : Type.{u2}} [_inst_1 : Primcodable.{u1} α] [_inst_2 : Primcodable.{u2} β] {e : Equiv.{succ u1, succ u2} α β} (q : β -> Prop), (Computable.{u2, u1} β α _inst_2 _inst_1 (coeFn.{max 1 (max (succ u2) (succ u1)) (succ u1) (succ u2), max (succ u2) (succ u1)} (Equiv.{succ u2, succ u1} β α) (fun (_x : Equiv.{succ u2, succ u1} β α) => β -> α) (Equiv.hasCoeToFun.{succ u2, succ u1} β α) (Equiv.symm.{succ u1, succ u2} α β e))) -> (OneOneReducible.{u2, u1} β α _inst_2 _inst_1 q (Function.comp.{succ u1, succ u2, 1} α β Prop q (coeFn.{max 1 (max (succ u1) (succ u2)) (succ u2) (succ u1), max (succ u1) (succ u2)} (Equiv.{succ u1, succ u2} α β) (fun (_x : Equiv.{succ u1, succ u2} α β) => α -> β) (Equiv.hasCoeToFun.{succ u1, succ u2} α β) e)))
+but is expected to have type
+  forall {α : Type.{u2}} {β : Type.{u1}} [_inst_1 : Primcodable.{u2} α] [_inst_2 : Primcodable.{u1} β] {e : Equiv.{succ u2, succ u1} α β} (q : β -> Prop), (Computable.{u1, u2} β α _inst_2 _inst_1 (FunLike.coe.{max (succ u2) (succ u1), succ u1, succ u2} (Equiv.{succ u1, succ u2} β α) β (fun (_x : β) => (fun (x._@.Mathlib.Logic.Equiv.Defs._hyg.808 : β) => α) _x) (Equiv.instFunLikeEquiv.{succ u1, succ u2} β α) (Equiv.symm.{succ u2, succ u1} α β e))) -> (OneOneReducible.{u1, u2} β α _inst_2 _inst_1 q (Function.comp.{succ u2, succ u1, 1} α β Prop q (FunLike.coe.{max (succ u2) (succ u1), succ u2, succ u1} (Equiv.{succ u2, succ u1} α β) α (fun (_x : α) => (fun (x._@.Mathlib.Logic.Equiv.Defs._hyg.808 : α) => β) _x) (Equiv.instFunLikeEquiv.{succ u2, succ u1} α β) e)))
+Case conversion may be inaccurate. Consider using '#align one_one_reducible.of_equiv_symm OneOneReducible.of_equiv_symmₓ'. -/
 theorem OneOneReducible.of_equiv_symm {α β} [Primcodable α] [Primcodable β] {e : α ≃ β}
     (q : β → Prop) (h : Computable e.symm) : q ≤₁ (q ∘ e) := by
   convert OneOneReducible.of_equiv _ h <;> funext <;> simp
 #align one_one_reducible.of_equiv_symm OneOneReducible.of_equiv_symm
 
+#print reflexive_oneOneReducible /-
 theorem reflexive_oneOneReducible {α} [Primcodable α] : Reflexive (@OneOneReducible α α _ _) :=
   oneOneReducible_refl
 #align reflexive_one_one_reducible reflexive_oneOneReducible
+-/
 
+#print transitive_oneOneReducible /-
 theorem transitive_oneOneReducible {α} [Primcodable α] : Transitive (@OneOneReducible α α _ _) :=
   fun p q r => OneOneReducible.trans
 #align transitive_one_one_reducible transitive_oneOneReducible
+-/
 
 namespace ComputablePred
 
@@ -131,6 +189,12 @@ variable [Primcodable α] [Primcodable β] [Primcodable σ]
 
 open Computable
 
+/- warning: computable_pred.computable_of_many_one_reducible -> ComputablePred.computable_of_manyOneReducible is a dubious translation:
+lean 3 declaration is
+  forall {α : Type.{u1}} {β : Type.{u2}} [_inst_1 : Primcodable.{u1} α] [_inst_2 : Primcodable.{u2} β] {p : α -> Prop} {q : β -> Prop}, (ManyOneReducible.{u1, u2} α β _inst_1 _inst_2 p q) -> (ComputablePred.{u2} β _inst_2 q) -> (ComputablePred.{u1} α _inst_1 p)
+but is expected to have type
+  forall {α : Type.{u2}} {β : Type.{u1}} [_inst_1 : Primcodable.{u2} α] [_inst_2 : Primcodable.{u1} β] {p : α -> Prop} {q : β -> Prop}, (ManyOneReducible.{u2, u1} α β _inst_1 _inst_2 p q) -> (ComputablePred.{u1} β _inst_2 q) -> (ComputablePred.{u2} α _inst_1 p)
+Case conversion may be inaccurate. Consider using '#align computable_pred.computable_of_many_one_reducible ComputablePred.computable_of_manyOneReducibleₓ'. -/
 theorem computable_of_manyOneReducible {p : α → Prop} {q : β → Prop} (h₁ : p ≤₀ q)
     (h₂ : ComputablePred q) : ComputablePred p :=
   by
@@ -140,6 +204,12 @@ theorem computable_of_manyOneReducible {p : α → Prop} {q : β → Prop} (h₁
   exact ⟨by infer_instance, by simpa using hg.comp c⟩
 #align computable_pred.computable_of_many_one_reducible ComputablePred.computable_of_manyOneReducible
 
+/- warning: computable_pred.computable_of_one_one_reducible -> ComputablePred.computable_of_oneOneReducible is a dubious translation:
+lean 3 declaration is
+  forall {α : Type.{u1}} {β : Type.{u2}} [_inst_1 : Primcodable.{u1} α] [_inst_2 : Primcodable.{u2} β] {p : α -> Prop} {q : β -> Prop}, (OneOneReducible.{u1, u2} α β _inst_1 _inst_2 p q) -> (ComputablePred.{u2} β _inst_2 q) -> (ComputablePred.{u1} α _inst_1 p)
+but is expected to have type
+  forall {α : Type.{u2}} {β : Type.{u1}} [_inst_1 : Primcodable.{u2} α] [_inst_2 : Primcodable.{u1} β] {p : α -> Prop} {q : β -> Prop}, (OneOneReducible.{u2, u1} α β _inst_1 _inst_2 p q) -> (ComputablePred.{u1} β _inst_2 q) -> (ComputablePred.{u2} α _inst_1 p)
+Case conversion may be inaccurate. Consider using '#align computable_pred.computable_of_one_one_reducible ComputablePred.computable_of_oneOneReducibleₓ'. -/
 theorem computable_of_oneOneReducible {p : α → Prop} {q : β → Prop} (h : p ≤₁ q) :
     ComputablePred q → ComputablePred p :=
   computable_of_manyOneReducible h.to_many_one
@@ -147,165 +217,311 @@ theorem computable_of_oneOneReducible {p : α → Prop} {q : β → Prop} (h : p
 
 end ComputablePred
 
+#print ManyOneEquiv /-
 /-- `p` and `q` are many-one equivalent if each one is many-one reducible to the other. -/
 def ManyOneEquiv {α β} [Primcodable α] [Primcodable β] (p : α → Prop) (q : β → Prop) :=
   p ≤₀ q ∧ q ≤₀ p
 #align many_one_equiv ManyOneEquiv
+-/
 
+#print OneOneEquiv /-
 /-- `p` and `q` are one-one equivalent if each one is one-one reducible to the other. -/
 def OneOneEquiv {α β} [Primcodable α] [Primcodable β] (p : α → Prop) (q : β → Prop) :=
   p ≤₁ q ∧ q ≤₁ p
 #align one_one_equiv OneOneEquiv
+-/
 
+#print manyOneEquiv_refl /-
 @[refl]
 theorem manyOneEquiv_refl {α} [Primcodable α] (p : α → Prop) : ManyOneEquiv p p :=
   ⟨manyOneReducible_refl _, manyOneReducible_refl _⟩
 #align many_one_equiv_refl manyOneEquiv_refl
+-/
 
+/- warning: many_one_equiv.symm -> ManyOneEquiv.symm is a dubious translation:
+lean 3 declaration is
+  forall {α : Type.{u1}} {β : Type.{u2}} [_inst_1 : Primcodable.{u1} α] [_inst_2 : Primcodable.{u2} β] {p : α -> Prop} {q : β -> Prop}, (ManyOneEquiv.{u1, u2} α β _inst_1 _inst_2 p q) -> (ManyOneEquiv.{u2, u1} β α _inst_2 _inst_1 q p)
+but is expected to have type
+  forall {α : Type.{u2}} {β : Type.{u1}} [_inst_1 : Primcodable.{u2} α] [_inst_2 : Primcodable.{u1} β] {p : α -> Prop} {q : β -> Prop}, (ManyOneEquiv.{u2, u1} α β _inst_1 _inst_2 p q) -> (ManyOneEquiv.{u1, u2} β α _inst_2 _inst_1 q p)
+Case conversion may be inaccurate. Consider using '#align many_one_equiv.symm ManyOneEquiv.symmₓ'. -/
 @[symm]
 theorem ManyOneEquiv.symm {α β} [Primcodable α] [Primcodable β] {p : α → Prop} {q : β → Prop} :
     ManyOneEquiv p q → ManyOneEquiv q p :=
   And.symm
 #align many_one_equiv.symm ManyOneEquiv.symm
 
+/- warning: many_one_equiv.trans -> ManyOneEquiv.trans is a dubious translation:
+lean 3 declaration is
+  forall {α : Type.{u1}} {β : Type.{u2}} {γ : Type.{u3}} [_inst_1 : Primcodable.{u1} α] [_inst_2 : Primcodable.{u2} β] [_inst_3 : Primcodable.{u3} γ] {p : α -> Prop} {q : β -> Prop} {r : γ -> Prop}, (ManyOneEquiv.{u1, u2} α β _inst_1 _inst_2 p q) -> (ManyOneEquiv.{u2, u3} β γ _inst_2 _inst_3 q r) -> (ManyOneEquiv.{u1, u3} α γ _inst_1 _inst_3 p r)
+but is expected to have type
+  forall {α : Type.{u3}} {β : Type.{u2}} {γ : Type.{u1}} [_inst_1 : Primcodable.{u3} α] [_inst_2 : Primcodable.{u2} β] [_inst_3 : Primcodable.{u1} γ] {p : α -> Prop} {q : β -> Prop} {r : γ -> Prop}, (ManyOneEquiv.{u3, u2} α β _inst_1 _inst_2 p q) -> (ManyOneEquiv.{u2, u1} β γ _inst_2 _inst_3 q r) -> (ManyOneEquiv.{u3, u1} α γ _inst_1 _inst_3 p r)
+Case conversion may be inaccurate. Consider using '#align many_one_equiv.trans ManyOneEquiv.transₓ'. -/
 @[trans]
 theorem ManyOneEquiv.trans {α β γ} [Primcodable α] [Primcodable β] [Primcodable γ] {p : α → Prop}
     {q : β → Prop} {r : γ → Prop} : ManyOneEquiv p q → ManyOneEquiv q r → ManyOneEquiv p r
   | ⟨pq, qp⟩, ⟨qr, rq⟩ => ⟨pq.trans qr, rq.trans qp⟩
 #align many_one_equiv.trans ManyOneEquiv.trans
 
+#print equivalence_of_manyOneEquiv /-
 theorem equivalence_of_manyOneEquiv {α} [Primcodable α] : Equivalence (@ManyOneEquiv α α _ _) :=
   ⟨manyOneEquiv_refl, fun x y => ManyOneEquiv.symm, fun x y z => ManyOneEquiv.trans⟩
 #align equivalence_of_many_one_equiv equivalence_of_manyOneEquiv
+-/
 
+#print oneOneEquiv_refl /-
 @[refl]
 theorem oneOneEquiv_refl {α} [Primcodable α] (p : α → Prop) : OneOneEquiv p p :=
   ⟨oneOneReducible_refl _, oneOneReducible_refl _⟩
 #align one_one_equiv_refl oneOneEquiv_refl
+-/
 
+/- warning: one_one_equiv.symm -> OneOneEquiv.symm is a dubious translation:
+lean 3 declaration is
+  forall {α : Type.{u1}} {β : Type.{u2}} [_inst_1 : Primcodable.{u1} α] [_inst_2 : Primcodable.{u2} β] {p : α -> Prop} {q : β -> Prop}, (OneOneEquiv.{u1, u2} α β _inst_1 _inst_2 p q) -> (OneOneEquiv.{u2, u1} β α _inst_2 _inst_1 q p)
+but is expected to have type
+  forall {α : Type.{u2}} {β : Type.{u1}} [_inst_1 : Primcodable.{u2} α] [_inst_2 : Primcodable.{u1} β] {p : α -> Prop} {q : β -> Prop}, (OneOneEquiv.{u2, u1} α β _inst_1 _inst_2 p q) -> (OneOneEquiv.{u1, u2} β α _inst_2 _inst_1 q p)
+Case conversion may be inaccurate. Consider using '#align one_one_equiv.symm OneOneEquiv.symmₓ'. -/
 @[symm]
 theorem OneOneEquiv.symm {α β} [Primcodable α] [Primcodable β] {p : α → Prop} {q : β → Prop} :
     OneOneEquiv p q → OneOneEquiv q p :=
   And.symm
 #align one_one_equiv.symm OneOneEquiv.symm
 
+/- warning: one_one_equiv.trans -> OneOneEquiv.trans is a dubious translation:
+lean 3 declaration is
+  forall {α : Type.{u1}} {β : Type.{u2}} {γ : Type.{u3}} [_inst_1 : Primcodable.{u1} α] [_inst_2 : Primcodable.{u2} β] [_inst_3 : Primcodable.{u3} γ] {p : α -> Prop} {q : β -> Prop} {r : γ -> Prop}, (OneOneEquiv.{u1, u2} α β _inst_1 _inst_2 p q) -> (OneOneEquiv.{u2, u3} β γ _inst_2 _inst_3 q r) -> (OneOneEquiv.{u1, u3} α γ _inst_1 _inst_3 p r)
+but is expected to have type
+  forall {α : Type.{u3}} {β : Type.{u2}} {γ : Type.{u1}} [_inst_1 : Primcodable.{u3} α] [_inst_2 : Primcodable.{u2} β] [_inst_3 : Primcodable.{u1} γ] {p : α -> Prop} {q : β -> Prop} {r : γ -> Prop}, (OneOneEquiv.{u3, u2} α β _inst_1 _inst_2 p q) -> (OneOneEquiv.{u2, u1} β γ _inst_2 _inst_3 q r) -> (OneOneEquiv.{u3, u1} α γ _inst_1 _inst_3 p r)
+Case conversion may be inaccurate. Consider using '#align one_one_equiv.trans OneOneEquiv.transₓ'. -/
 @[trans]
 theorem OneOneEquiv.trans {α β γ} [Primcodable α] [Primcodable β] [Primcodable γ] {p : α → Prop}
     {q : β → Prop} {r : γ → Prop} : OneOneEquiv p q → OneOneEquiv q r → OneOneEquiv p r
   | ⟨pq, qp⟩, ⟨qr, rq⟩ => ⟨pq.trans qr, rq.trans qp⟩
 #align one_one_equiv.trans OneOneEquiv.trans
 
+#print equivalence_of_oneOneEquiv /-
 theorem equivalence_of_oneOneEquiv {α} [Primcodable α] : Equivalence (@OneOneEquiv α α _ _) :=
   ⟨oneOneEquiv_refl, fun x y => OneOneEquiv.symm, fun x y z => OneOneEquiv.trans⟩
 #align equivalence_of_one_one_equiv equivalence_of_oneOneEquiv
+-/
 
+/- warning: one_one_equiv.to_many_one -> OneOneEquiv.to_many_one is a dubious translation:
+lean 3 declaration is
+  forall {α : Type.{u1}} {β : Type.{u2}} [_inst_1 : Primcodable.{u1} α] [_inst_2 : Primcodable.{u2} β] {p : α -> Prop} {q : β -> Prop}, (OneOneEquiv.{u1, u2} α β _inst_1 _inst_2 p q) -> (ManyOneEquiv.{u1, u2} α β _inst_1 _inst_2 p q)
+but is expected to have type
+  forall {α : Type.{u2}} {β : Type.{u1}} [_inst_1 : Primcodable.{u2} α] [_inst_2 : Primcodable.{u1} β] {p : α -> Prop} {q : β -> Prop}, (OneOneEquiv.{u2, u1} α β _inst_1 _inst_2 p q) -> (ManyOneEquiv.{u2, u1} α β _inst_1 _inst_2 p q)
+Case conversion may be inaccurate. Consider using '#align one_one_equiv.to_many_one OneOneEquiv.to_many_oneₓ'. -/
 theorem OneOneEquiv.to_many_one {α β} [Primcodable α] [Primcodable β] {p : α → Prop}
     {q : β → Prop} : OneOneEquiv p q → ManyOneEquiv p q
   | ⟨pq, qp⟩ => ⟨pq.to_many_one, qp.to_many_one⟩
 #align one_one_equiv.to_many_one OneOneEquiv.to_many_one
 
+#print Equiv.Computable /-
 /-- a computable bijection -/
 def Equiv.Computable {α β} [Primcodable α] [Primcodable β] (e : α ≃ β) :=
   Computable e ∧ Computable e.symm
 #align equiv.computable Equiv.Computable
+-/
 
+/- warning: equiv.computable.symm -> Equiv.Computable.symm is a dubious translation:
+lean 3 declaration is
+  forall {α : Type.{u1}} {β : Type.{u2}} [_inst_1 : Primcodable.{u1} α] [_inst_2 : Primcodable.{u2} β] {e : Equiv.{succ u1, succ u2} α β}, (Equiv.Computable.{u1, u2} α β _inst_1 _inst_2 e) -> (Equiv.Computable.{u2, u1} β α _inst_2 _inst_1 (Equiv.symm.{succ u1, succ u2} α β e))
+but is expected to have type
+  forall {α : Type.{u2}} {β : Type.{u1}} [_inst_1 : Primcodable.{u2} α] [_inst_2 : Primcodable.{u1} β] {e : Equiv.{succ u2, succ u1} α β}, (Equiv.Computable.{u2, u1} α β _inst_1 _inst_2 e) -> (Equiv.Computable.{u1, u2} β α _inst_2 _inst_1 (Equiv.symm.{succ u2, succ u1} α β e))
+Case conversion may be inaccurate. Consider using '#align equiv.computable.symm Equiv.Computable.symmₓ'. -/
 theorem Equiv.Computable.symm {α β} [Primcodable α] [Primcodable β] {e : α ≃ β} :
     e.Computable → e.symm.Computable :=
   And.symm
 #align equiv.computable.symm Equiv.Computable.symm
 
+/- warning: equiv.computable.trans -> Equiv.Computable.trans is a dubious translation:
+lean 3 declaration is
+  forall {α : Type.{u1}} {β : Type.{u2}} {γ : Type.{u3}} [_inst_1 : Primcodable.{u1} α] [_inst_2 : Primcodable.{u2} β] [_inst_3 : Primcodable.{u3} γ] {e₁ : Equiv.{succ u1, succ u2} α β} {e₂ : Equiv.{succ u2, succ u3} β γ}, (Equiv.Computable.{u1, u2} α β _inst_1 _inst_2 e₁) -> (Equiv.Computable.{u2, u3} β γ _inst_2 _inst_3 e₂) -> (Equiv.Computable.{u1, u3} α γ _inst_1 _inst_3 (Equiv.trans.{succ u1, succ u2, succ u3} α β γ e₁ e₂))
+but is expected to have type
+  forall {α : Type.{u3}} {β : Type.{u2}} {γ : Type.{u1}} [_inst_1 : Primcodable.{u3} α] [_inst_2 : Primcodable.{u2} β] [_inst_3 : Primcodable.{u1} γ] {e₁ : Equiv.{succ u3, succ u2} α β} {e₂ : Equiv.{succ u2, succ u1} β γ}, (Equiv.Computable.{u3, u2} α β _inst_1 _inst_2 e₁) -> (Equiv.Computable.{u2, u1} β γ _inst_2 _inst_3 e₂) -> (Equiv.Computable.{u3, u1} α γ _inst_1 _inst_3 (Equiv.trans.{succ u3, succ u2, succ u1} α β γ e₁ e₂))
+Case conversion may be inaccurate. Consider using '#align equiv.computable.trans Equiv.Computable.transₓ'. -/
 theorem Equiv.Computable.trans {α β γ} [Primcodable α] [Primcodable β] [Primcodable γ] {e₁ : α ≃ β}
     {e₂ : β ≃ γ} : e₁.Computable → e₂.Computable → (e₁.trans e₂).Computable
   | ⟨l₁, r₁⟩, ⟨l₂, r₂⟩ => ⟨l₂.comp l₁, r₁.comp r₂⟩
 #align equiv.computable.trans Equiv.Computable.trans
 
+#print Computable.eqv /-
 theorem Computable.eqv (α) [Denumerable α] : (Denumerable.eqv α).Computable :=
   ⟨Computable.encode, Computable.ofNat _⟩
 #align computable.eqv Computable.eqv
+-/
 
+/- warning: computable.equiv₂ -> Computable.equiv₂ is a dubious translation:
+lean 3 declaration is
+  forall (α : Type.{u1}) (β : Type.{u2}) [_inst_1 : Denumerable.{u1} α] [_inst_2 : Denumerable.{u2} β], Equiv.Computable.{u1, u2} α β (Primcodable.ofDenumerable.{u1} α _inst_1) (Primcodable.ofDenumerable.{u2} β _inst_2) (Denumerable.equiv₂.{u1, u2} α β _inst_1 _inst_2)
+but is expected to have type
+  forall (α : Type.{u2}) (β : Type.{u1}) [_inst_1 : Denumerable.{u2} α] [_inst_2 : Denumerable.{u1} β], Equiv.Computable.{u2, u1} α β (Primcodable.ofDenumerable.{u2} α _inst_1) (Primcodable.ofDenumerable.{u1} β _inst_2) (Denumerable.equiv₂.{u2, u1} α β _inst_1 _inst_2)
+Case conversion may be inaccurate. Consider using '#align computable.equiv₂ Computable.equiv₂ₓ'. -/
 theorem Computable.equiv₂ (α β) [Denumerable α] [Denumerable β] :
     (Denumerable.equiv₂ α β).Computable :=
   (Computable.eqv _).trans (Computable.eqv _).symm
 #align computable.equiv₂ Computable.equiv₂
 
+/- warning: one_one_equiv.of_equiv -> OneOneEquiv.of_equiv is a dubious translation:
+lean 3 declaration is
+  forall {α : Type.{u1}} {β : Type.{u2}} [_inst_1 : Primcodable.{u1} α] [_inst_2 : Primcodable.{u2} β] {e : Equiv.{succ u1, succ u2} α β}, (Equiv.Computable.{u1, u2} α β _inst_1 _inst_2 e) -> (forall {p : β -> Prop}, OneOneEquiv.{u1, u2} α β _inst_1 _inst_2 (Function.comp.{succ u1, succ u2, 1} α β Prop p (coeFn.{max 1 (max (succ u1) (succ u2)) (succ u2) (succ u1), max (succ u1) (succ u2)} (Equiv.{succ u1, succ u2} α β) (fun (_x : Equiv.{succ u1, succ u2} α β) => α -> β) (Equiv.hasCoeToFun.{succ u1, succ u2} α β) e)) p)
+but is expected to have type
+  forall {α : Type.{u2}} {β : Type.{u1}} [_inst_1 : Primcodable.{u2} α] [_inst_2 : Primcodable.{u1} β] {e : Equiv.{succ u2, succ u1} α β}, (Equiv.Computable.{u2, u1} α β _inst_1 _inst_2 e) -> (forall {p : β -> Prop}, OneOneEquiv.{u2, u1} α β _inst_1 _inst_2 (Function.comp.{succ u2, succ u1, 1} α β Prop p (FunLike.coe.{max (succ u2) (succ u1), succ u2, succ u1} (Equiv.{succ u2, succ u1} α β) α (fun (_x : α) => (fun (x._@.Mathlib.Logic.Equiv.Defs._hyg.808 : α) => β) _x) (Equiv.instFunLikeEquiv.{succ u2, succ u1} α β) e)) p)
+Case conversion may be inaccurate. Consider using '#align one_one_equiv.of_equiv OneOneEquiv.of_equivₓ'. -/
 theorem OneOneEquiv.of_equiv {α β} [Primcodable α] [Primcodable β] {e : α ≃ β} (h : e.Computable)
     {p} : OneOneEquiv (p ∘ e) p :=
   ⟨OneOneReducible.of_equiv _ h.1, OneOneReducible.of_equiv_symm _ h.2⟩
 #align one_one_equiv.of_equiv OneOneEquiv.of_equiv
 
+/- warning: many_one_equiv.of_equiv -> ManyOneEquiv.of_equiv is a dubious translation:
+lean 3 declaration is
+  forall {α : Type.{u1}} {β : Type.{u2}} [_inst_1 : Primcodable.{u1} α] [_inst_2 : Primcodable.{u2} β] {e : Equiv.{succ u1, succ u2} α β}, (Equiv.Computable.{u1, u2} α β _inst_1 _inst_2 e) -> (forall {p : β -> Prop}, ManyOneEquiv.{u1, u2} α β _inst_1 _inst_2 (Function.comp.{succ u1, succ u2, 1} α β Prop p (coeFn.{max 1 (max (succ u1) (succ u2)) (succ u2) (succ u1), max (succ u1) (succ u2)} (Equiv.{succ u1, succ u2} α β) (fun (_x : Equiv.{succ u1, succ u2} α β) => α -> β) (Equiv.hasCoeToFun.{succ u1, succ u2} α β) e)) p)
+but is expected to have type
+  forall {α : Type.{u2}} {β : Type.{u1}} [_inst_1 : Primcodable.{u2} α] [_inst_2 : Primcodable.{u1} β] {e : Equiv.{succ u2, succ u1} α β}, (Equiv.Computable.{u2, u1} α β _inst_1 _inst_2 e) -> (forall {p : β -> Prop}, ManyOneEquiv.{u2, u1} α β _inst_1 _inst_2 (Function.comp.{succ u2, succ u1, 1} α β Prop p (FunLike.coe.{max (succ u2) (succ u1), succ u2, succ u1} (Equiv.{succ u2, succ u1} α β) α (fun (_x : α) => (fun (x._@.Mathlib.Logic.Equiv.Defs._hyg.808 : α) => β) _x) (Equiv.instFunLikeEquiv.{succ u2, succ u1} α β) e)) p)
+Case conversion may be inaccurate. Consider using '#align many_one_equiv.of_equiv ManyOneEquiv.of_equivₓ'. -/
 theorem ManyOneEquiv.of_equiv {α β} [Primcodable α] [Primcodable β] {e : α ≃ β} (h : e.Computable)
     {p} : ManyOneEquiv (p ∘ e) p :=
   (OneOneEquiv.of_equiv h).to_many_one
 #align many_one_equiv.of_equiv ManyOneEquiv.of_equiv
 
+/- warning: many_one_equiv.le_congr_left -> ManyOneEquiv.le_congr_left is a dubious translation:
+lean 3 declaration is
+  forall {α : Type.{u1}} {β : Type.{u2}} {γ : Type.{u3}} [_inst_1 : Primcodable.{u1} α] [_inst_2 : Primcodable.{u2} β] [_inst_3 : Primcodable.{u3} γ] {p : α -> Prop} {q : β -> Prop} {r : γ -> Prop}, (ManyOneEquiv.{u1, u2} α β _inst_1 _inst_2 p q) -> (Iff (ManyOneReducible.{u1, u3} α γ _inst_1 _inst_3 p r) (ManyOneReducible.{u2, u3} β γ _inst_2 _inst_3 q r))
+but is expected to have type
+  forall {α : Type.{u3}} {β : Type.{u2}} {γ : Type.{u1}} [_inst_1 : Primcodable.{u3} α] [_inst_2 : Primcodable.{u2} β] [_inst_3 : Primcodable.{u1} γ] {p : α -> Prop} {q : β -> Prop} {r : γ -> Prop}, (ManyOneEquiv.{u3, u2} α β _inst_1 _inst_2 p q) -> (Iff (ManyOneReducible.{u3, u1} α γ _inst_1 _inst_3 p r) (ManyOneReducible.{u2, u1} β γ _inst_2 _inst_3 q r))
+Case conversion may be inaccurate. Consider using '#align many_one_equiv.le_congr_left ManyOneEquiv.le_congr_leftₓ'. -/
 theorem ManyOneEquiv.le_congr_left {α β γ} [Primcodable α] [Primcodable β] [Primcodable γ]
     {p : α → Prop} {q : β → Prop} {r : γ → Prop} (h : ManyOneEquiv p q) : p ≤₀ r ↔ q ≤₀ r :=
   ⟨h.2.trans, h.1.trans⟩
 #align many_one_equiv.le_congr_left ManyOneEquiv.le_congr_left
 
+/- warning: many_one_equiv.le_congr_right -> ManyOneEquiv.le_congr_right is a dubious translation:
+lean 3 declaration is
+  forall {α : Type.{u1}} {β : Type.{u2}} {γ : Type.{u3}} [_inst_1 : Primcodable.{u1} α] [_inst_2 : Primcodable.{u2} β] [_inst_3 : Primcodable.{u3} γ] {p : α -> Prop} {q : β -> Prop} {r : γ -> Prop}, (ManyOneEquiv.{u2, u3} β γ _inst_2 _inst_3 q r) -> (Iff (ManyOneReducible.{u1, u2} α β _inst_1 _inst_2 p q) (ManyOneReducible.{u1, u3} α γ _inst_1 _inst_3 p r))
+but is expected to have type
+  forall {α : Type.{u3}} {β : Type.{u2}} {γ : Type.{u1}} [_inst_1 : Primcodable.{u3} α] [_inst_2 : Primcodable.{u2} β] [_inst_3 : Primcodable.{u1} γ] {p : α -> Prop} {q : β -> Prop} {r : γ -> Prop}, (ManyOneEquiv.{u2, u1} β γ _inst_2 _inst_3 q r) -> (Iff (ManyOneReducible.{u3, u2} α β _inst_1 _inst_2 p q) (ManyOneReducible.{u3, u1} α γ _inst_1 _inst_3 p r))
+Case conversion may be inaccurate. Consider using '#align many_one_equiv.le_congr_right ManyOneEquiv.le_congr_rightₓ'. -/
 theorem ManyOneEquiv.le_congr_right {α β γ} [Primcodable α] [Primcodable β] [Primcodable γ]
     {p : α → Prop} {q : β → Prop} {r : γ → Prop} (h : ManyOneEquiv q r) : p ≤₀ q ↔ p ≤₀ r :=
   ⟨fun h' => h'.trans h.1, fun h' => h'.trans h.2⟩
 #align many_one_equiv.le_congr_right ManyOneEquiv.le_congr_right
 
+/- warning: one_one_equiv.le_congr_left -> OneOneEquiv.le_congr_left is a dubious translation:
+lean 3 declaration is
+  forall {α : Type.{u1}} {β : Type.{u2}} {γ : Type.{u3}} [_inst_1 : Primcodable.{u1} α] [_inst_2 : Primcodable.{u2} β] [_inst_3 : Primcodable.{u3} γ] {p : α -> Prop} {q : β -> Prop} {r : γ -> Prop}, (OneOneEquiv.{u1, u2} α β _inst_1 _inst_2 p q) -> (Iff (OneOneReducible.{u1, u3} α γ _inst_1 _inst_3 p r) (OneOneReducible.{u2, u3} β γ _inst_2 _inst_3 q r))
+but is expected to have type
+  forall {α : Type.{u3}} {β : Type.{u2}} {γ : Type.{u1}} [_inst_1 : Primcodable.{u3} α] [_inst_2 : Primcodable.{u2} β] [_inst_3 : Primcodable.{u1} γ] {p : α -> Prop} {q : β -> Prop} {r : γ -> Prop}, (OneOneEquiv.{u3, u2} α β _inst_1 _inst_2 p q) -> (Iff (OneOneReducible.{u3, u1} α γ _inst_1 _inst_3 p r) (OneOneReducible.{u2, u1} β γ _inst_2 _inst_3 q r))
+Case conversion may be inaccurate. Consider using '#align one_one_equiv.le_congr_left OneOneEquiv.le_congr_leftₓ'. -/
 theorem OneOneEquiv.le_congr_left {α β γ} [Primcodable α] [Primcodable β] [Primcodable γ]
     {p : α → Prop} {q : β → Prop} {r : γ → Prop} (h : OneOneEquiv p q) : p ≤₁ r ↔ q ≤₁ r :=
   ⟨h.2.trans, h.1.trans⟩
 #align one_one_equiv.le_congr_left OneOneEquiv.le_congr_left
 
+/- warning: one_one_equiv.le_congr_right -> OneOneEquiv.le_congr_right is a dubious translation:
+lean 3 declaration is
+  forall {α : Type.{u1}} {β : Type.{u2}} {γ : Type.{u3}} [_inst_1 : Primcodable.{u1} α] [_inst_2 : Primcodable.{u2} β] [_inst_3 : Primcodable.{u3} γ] {p : α -> Prop} {q : β -> Prop} {r : γ -> Prop}, (OneOneEquiv.{u2, u3} β γ _inst_2 _inst_3 q r) -> (Iff (OneOneReducible.{u1, u2} α β _inst_1 _inst_2 p q) (OneOneReducible.{u1, u3} α γ _inst_1 _inst_3 p r))
+but is expected to have type
+  forall {α : Type.{u3}} {β : Type.{u2}} {γ : Type.{u1}} [_inst_1 : Primcodable.{u3} α] [_inst_2 : Primcodable.{u2} β] [_inst_3 : Primcodable.{u1} γ] {p : α -> Prop} {q : β -> Prop} {r : γ -> Prop}, (OneOneEquiv.{u2, u1} β γ _inst_2 _inst_3 q r) -> (Iff (OneOneReducible.{u3, u2} α β _inst_1 _inst_2 p q) (OneOneReducible.{u3, u1} α γ _inst_1 _inst_3 p r))
+Case conversion may be inaccurate. Consider using '#align one_one_equiv.le_congr_right OneOneEquiv.le_congr_rightₓ'. -/
 theorem OneOneEquiv.le_congr_right {α β γ} [Primcodable α] [Primcodable β] [Primcodable γ]
     {p : α → Prop} {q : β → Prop} {r : γ → Prop} (h : OneOneEquiv q r) : p ≤₁ q ↔ p ≤₁ r :=
   ⟨fun h' => h'.trans h.1, fun h' => h'.trans h.2⟩
 #align one_one_equiv.le_congr_right OneOneEquiv.le_congr_right
 
+/- warning: many_one_equiv.congr_left -> ManyOneEquiv.congr_left is a dubious translation:
+lean 3 declaration is
+  forall {α : Type.{u1}} {β : Type.{u2}} {γ : Type.{u3}} [_inst_1 : Primcodable.{u1} α] [_inst_2 : Primcodable.{u2} β] [_inst_3 : Primcodable.{u3} γ] {p : α -> Prop} {q : β -> Prop} {r : γ -> Prop}, (ManyOneEquiv.{u1, u2} α β _inst_1 _inst_2 p q) -> (Iff (ManyOneEquiv.{u1, u3} α γ _inst_1 _inst_3 p r) (ManyOneEquiv.{u2, u3} β γ _inst_2 _inst_3 q r))
+but is expected to have type
+  forall {α : Type.{u3}} {β : Type.{u2}} {γ : Type.{u1}} [_inst_1 : Primcodable.{u3} α] [_inst_2 : Primcodable.{u2} β] [_inst_3 : Primcodable.{u1} γ] {p : α -> Prop} {q : β -> Prop} {r : γ -> Prop}, (ManyOneEquiv.{u3, u2} α β _inst_1 _inst_2 p q) -> (Iff (ManyOneEquiv.{u3, u1} α γ _inst_1 _inst_3 p r) (ManyOneEquiv.{u2, u1} β γ _inst_2 _inst_3 q r))
+Case conversion may be inaccurate. Consider using '#align many_one_equiv.congr_left ManyOneEquiv.congr_leftₓ'. -/
 theorem ManyOneEquiv.congr_left {α β γ} [Primcodable α] [Primcodable β] [Primcodable γ]
     {p : α → Prop} {q : β → Prop} {r : γ → Prop} (h : ManyOneEquiv p q) :
     ManyOneEquiv p r ↔ ManyOneEquiv q r :=
   and_congr h.le_congr_left h.le_congr_right
 #align many_one_equiv.congr_left ManyOneEquiv.congr_left
 
+/- warning: many_one_equiv.congr_right -> ManyOneEquiv.congr_right is a dubious translation:
+lean 3 declaration is
+  forall {α : Type.{u1}} {β : Type.{u2}} {γ : Type.{u3}} [_inst_1 : Primcodable.{u1} α] [_inst_2 : Primcodable.{u2} β] [_inst_3 : Primcodable.{u3} γ] {p : α -> Prop} {q : β -> Prop} {r : γ -> Prop}, (ManyOneEquiv.{u2, u3} β γ _inst_2 _inst_3 q r) -> (Iff (ManyOneEquiv.{u1, u2} α β _inst_1 _inst_2 p q) (ManyOneEquiv.{u1, u3} α γ _inst_1 _inst_3 p r))
+but is expected to have type
+  forall {α : Type.{u3}} {β : Type.{u2}} {γ : Type.{u1}} [_inst_1 : Primcodable.{u3} α] [_inst_2 : Primcodable.{u2} β] [_inst_3 : Primcodable.{u1} γ] {p : α -> Prop} {q : β -> Prop} {r : γ -> Prop}, (ManyOneEquiv.{u2, u1} β γ _inst_2 _inst_3 q r) -> (Iff (ManyOneEquiv.{u3, u2} α β _inst_1 _inst_2 p q) (ManyOneEquiv.{u3, u1} α γ _inst_1 _inst_3 p r))
+Case conversion may be inaccurate. Consider using '#align many_one_equiv.congr_right ManyOneEquiv.congr_rightₓ'. -/
 theorem ManyOneEquiv.congr_right {α β γ} [Primcodable α] [Primcodable β] [Primcodable γ]
     {p : α → Prop} {q : β → Prop} {r : γ → Prop} (h : ManyOneEquiv q r) :
     ManyOneEquiv p q ↔ ManyOneEquiv p r :=
   and_congr h.le_congr_right h.le_congr_left
 #align many_one_equiv.congr_right ManyOneEquiv.congr_right
 
+/- warning: one_one_equiv.congr_left -> OneOneEquiv.congr_left is a dubious translation:
+lean 3 declaration is
+  forall {α : Type.{u1}} {β : Type.{u2}} {γ : Type.{u3}} [_inst_1 : Primcodable.{u1} α] [_inst_2 : Primcodable.{u2} β] [_inst_3 : Primcodable.{u3} γ] {p : α -> Prop} {q : β -> Prop} {r : γ -> Prop}, (OneOneEquiv.{u1, u2} α β _inst_1 _inst_2 p q) -> (Iff (OneOneEquiv.{u1, u3} α γ _inst_1 _inst_3 p r) (OneOneEquiv.{u2, u3} β γ _inst_2 _inst_3 q r))
+but is expected to have type
+  forall {α : Type.{u3}} {β : Type.{u2}} {γ : Type.{u1}} [_inst_1 : Primcodable.{u3} α] [_inst_2 : Primcodable.{u2} β] [_inst_3 : Primcodable.{u1} γ] {p : α -> Prop} {q : β -> Prop} {r : γ -> Prop}, (OneOneEquiv.{u3, u2} α β _inst_1 _inst_2 p q) -> (Iff (OneOneEquiv.{u3, u1} α γ _inst_1 _inst_3 p r) (OneOneEquiv.{u2, u1} β γ _inst_2 _inst_3 q r))
+Case conversion may be inaccurate. Consider using '#align one_one_equiv.congr_left OneOneEquiv.congr_leftₓ'. -/
 theorem OneOneEquiv.congr_left {α β γ} [Primcodable α] [Primcodable β] [Primcodable γ]
     {p : α → Prop} {q : β → Prop} {r : γ → Prop} (h : OneOneEquiv p q) :
     OneOneEquiv p r ↔ OneOneEquiv q r :=
   and_congr h.le_congr_left h.le_congr_right
 #align one_one_equiv.congr_left OneOneEquiv.congr_left
 
+/- warning: one_one_equiv.congr_right -> OneOneEquiv.congr_right is a dubious translation:
+lean 3 declaration is
+  forall {α : Type.{u1}} {β : Type.{u2}} {γ : Type.{u3}} [_inst_1 : Primcodable.{u1} α] [_inst_2 : Primcodable.{u2} β] [_inst_3 : Primcodable.{u3} γ] {p : α -> Prop} {q : β -> Prop} {r : γ -> Prop}, (OneOneEquiv.{u2, u3} β γ _inst_2 _inst_3 q r) -> (Iff (OneOneEquiv.{u1, u2} α β _inst_1 _inst_2 p q) (OneOneEquiv.{u1, u3} α γ _inst_1 _inst_3 p r))
+but is expected to have type
+  forall {α : Type.{u3}} {β : Type.{u2}} {γ : Type.{u1}} [_inst_1 : Primcodable.{u3} α] [_inst_2 : Primcodable.{u2} β] [_inst_3 : Primcodable.{u1} γ] {p : α -> Prop} {q : β -> Prop} {r : γ -> Prop}, (OneOneEquiv.{u2, u1} β γ _inst_2 _inst_3 q r) -> (Iff (OneOneEquiv.{u3, u2} α β _inst_1 _inst_2 p q) (OneOneEquiv.{u3, u1} α γ _inst_1 _inst_3 p r))
+Case conversion may be inaccurate. Consider using '#align one_one_equiv.congr_right OneOneEquiv.congr_rightₓ'. -/
 theorem OneOneEquiv.congr_right {α β γ} [Primcodable α] [Primcodable β] [Primcodable γ]
     {p : α → Prop} {q : β → Prop} {r : γ → Prop} (h : OneOneEquiv q r) :
     OneOneEquiv p q ↔ OneOneEquiv p r :=
   and_congr h.le_congr_right h.le_congr_left
 #align one_one_equiv.congr_right OneOneEquiv.congr_right
 
+#print Ulower.down_computable /-
 @[simp]
 theorem Ulower.down_computable {α} [Primcodable α] : (Ulower.equiv α).Computable :=
   ⟨Primrec.ulower_down.to_comp, Primrec.ulower_up.to_comp⟩
 #align ulower.down_computable Ulower.down_computable
+-/
 
+#print manyOneEquiv_up /-
 theorem manyOneEquiv_up {α} [Primcodable α] {p : α → Prop} : ManyOneEquiv (p ∘ Ulower.up) p :=
   ManyOneEquiv.of_equiv Ulower.down_computable.symm
 #align many_one_equiv_up manyOneEquiv_up
+-/
 
 -- mathport name: «expr ⊕' »
 local infixl:1001 " ⊕' " => Sum.elim
 
 open Nat.Primrec
 
+/- warning: one_one_reducible.disjoin_left -> OneOneReducible.disjoin_left is a dubious translation:
+lean 3 declaration is
+  forall {α : Type.{u1}} {β : Type.{u2}} [_inst_1 : Primcodable.{u1} α] [_inst_2 : Primcodable.{u2} β] {p : α -> Prop} {q : β -> Prop}, OneOneReducible.{u1, max u1 u2} α (Sum.{u1, u2} α β) _inst_1 (Primcodable.sum.{u1, u2} α β _inst_1 _inst_2) p (Sum.elim.{u1, u2, 1} α β Prop p q)
+but is expected to have type
+  forall {α : Type.{u2}} {β : Type.{u1}} [_inst_1 : Primcodable.{u2} α] [_inst_2 : Primcodable.{u1} β] {p : α -> Prop} {q : β -> Prop}, OneOneReducible.{u2, max u1 u2} α (Sum.{u2, u1} α β) _inst_1 (Primcodable.sum.{u2, u1} α β _inst_1 _inst_2) p (Sum.elim.{u2, u1, 1} α β Prop p q)
+Case conversion may be inaccurate. Consider using '#align one_one_reducible.disjoin_left OneOneReducible.disjoin_leftₓ'. -/
 theorem OneOneReducible.disjoin_left {α β} [Primcodable α] [Primcodable β] {p : α → Prop}
     {q : β → Prop} : p ≤₁ p ⊕' q :=
   ⟨Sum.inl, Computable.sum_inl, fun x y => Sum.inl.inj_iff.1, fun a => Iff.rfl⟩
 #align one_one_reducible.disjoin_left OneOneReducible.disjoin_left
 
+/- warning: one_one_reducible.disjoin_right -> OneOneReducible.disjoin_right is a dubious translation:
+lean 3 declaration is
+  forall {α : Type.{u1}} {β : Type.{u2}} [_inst_1 : Primcodable.{u1} α] [_inst_2 : Primcodable.{u2} β] {p : α -> Prop} {q : β -> Prop}, OneOneReducible.{u2, max u1 u2} β (Sum.{u1, u2} α β) _inst_2 (Primcodable.sum.{u1, u2} α β _inst_1 _inst_2) q (Sum.elim.{u1, u2, 1} α β Prop p q)
+but is expected to have type
+  forall {α : Type.{u2}} {β : Type.{u1}} [_inst_1 : Primcodable.{u2} α] [_inst_2 : Primcodable.{u1} β] {p : α -> Prop} {q : β -> Prop}, OneOneReducible.{u1, max u1 u2} β (Sum.{u2, u1} α β) _inst_2 (Primcodable.sum.{u2, u1} α β _inst_1 _inst_2) q (Sum.elim.{u2, u1, 1} α β Prop p q)
+Case conversion may be inaccurate. Consider using '#align one_one_reducible.disjoin_right OneOneReducible.disjoin_rightₓ'. -/
 theorem OneOneReducible.disjoin_right {α β} [Primcodable α] [Primcodable β] {p : α → Prop}
     {q : β → Prop} : q ≤₁ p ⊕' q :=
   ⟨Sum.inr, Computable.sum_inr, fun x y => Sum.inr.inj_iff.1, fun a => Iff.rfl⟩
 #align one_one_reducible.disjoin_right OneOneReducible.disjoin_right
 
+/- warning: disjoin_many_one_reducible -> disjoin_manyOneReducible is a dubious translation:
+lean 3 declaration is
+  forall {α : Type.{u1}} {β : Type.{u2}} {γ : Type.{u3}} [_inst_1 : Primcodable.{u1} α] [_inst_2 : Primcodable.{u2} β] [_inst_3 : Primcodable.{u3} γ] {p : α -> Prop} {q : β -> Prop} {r : γ -> Prop}, (ManyOneReducible.{u1, u3} α γ _inst_1 _inst_3 p r) -> (ManyOneReducible.{u2, u3} β γ _inst_2 _inst_3 q r) -> (ManyOneReducible.{max u1 u2, u3} (Sum.{u1, u2} α β) γ (Primcodable.sum.{u1, u2} α β _inst_1 _inst_2) _inst_3 (Sum.elim.{u1, u2, 1} α β Prop p q) r)
+but is expected to have type
+  forall {α : Type.{u3}} {β : Type.{u2}} {γ : Type.{u1}} [_inst_1 : Primcodable.{u3} α] [_inst_2 : Primcodable.{u2} β] [_inst_3 : Primcodable.{u1} γ] {p : α -> Prop} {q : β -> Prop} {r : γ -> Prop}, (ManyOneReducible.{u3, u1} α γ _inst_1 _inst_3 p r) -> (ManyOneReducible.{u2, u1} β γ _inst_2 _inst_3 q r) -> (ManyOneReducible.{max u2 u3, u1} (Sum.{u3, u2} α β) γ (Primcodable.sum.{u3, u2} α β _inst_1 _inst_2) _inst_3 (Sum.elim.{u3, u2, 1} α β Prop p q) r)
+Case conversion may be inaccurate. Consider using '#align disjoin_many_one_reducible disjoin_manyOneReducibleₓ'. -/
 theorem disjoin_manyOneReducible {α β γ} [Primcodable α] [Primcodable β] [Primcodable γ]
     {p : α → Prop} {q : β → Prop} {r : γ → Prop} : p ≤₀ r → q ≤₀ r → p ⊕' q ≤₀ r
   | ⟨f, c₁, h₁⟩, ⟨g, c₂, h₂⟩ =>
@@ -314,6 +530,12 @@ theorem disjoin_manyOneReducible {α β γ} [Primcodable α] [Primcodable β] [P
       by cases x <;> [apply h₁, apply h₂]⟩
 #align disjoin_many_one_reducible disjoin_manyOneReducible
 
+/- warning: disjoin_le -> disjoin_le is a dubious translation:
+lean 3 declaration is
+  forall {α : Type.{u1}} {β : Type.{u2}} {γ : Type.{u3}} [_inst_1 : Primcodable.{u1} α] [_inst_2 : Primcodable.{u2} β] [_inst_3 : Primcodable.{u3} γ] {p : α -> Prop} {q : β -> Prop} {r : γ -> Prop}, Iff (ManyOneReducible.{max u1 u2, u3} (Sum.{u1, u2} α β) γ (Primcodable.sum.{u1, u2} α β _inst_1 _inst_2) _inst_3 (Sum.elim.{u1, u2, 1} α β Prop p q) r) (And (ManyOneReducible.{u1, u3} α γ _inst_1 _inst_3 p r) (ManyOneReducible.{u2, u3} β γ _inst_2 _inst_3 q r))
+but is expected to have type
+  forall {α : Type.{u3}} {β : Type.{u2}} {γ : Type.{u1}} [_inst_1 : Primcodable.{u3} α] [_inst_2 : Primcodable.{u2} β] [_inst_3 : Primcodable.{u1} γ] {p : α -> Prop} {q : β -> Prop} {r : γ -> Prop}, Iff (ManyOneReducible.{max u2 u3, u1} (Sum.{u3, u2} α β) γ (Primcodable.sum.{u3, u2} α β _inst_1 _inst_2) _inst_3 (Sum.elim.{u3, u2, 1} α β Prop p q) r) (And (ManyOneReducible.{u3, u1} α γ _inst_1 _inst_3 p r) (ManyOneReducible.{u2, u1} β γ _inst_2 _inst_3 q r))
+Case conversion may be inaccurate. Consider using '#align disjoin_le disjoin_leₓ'. -/
 theorem disjoin_le {α β γ} [Primcodable α] [Primcodable β] [Primcodable γ] {p : α → Prop}
     {q : β → Prop} {r : γ → Prop} : p ⊕' q ≤₀ r ↔ p ≤₀ r ∧ q ≤₀ r :=
   ⟨fun h =>
@@ -328,56 +550,75 @@ variable {β : Type v} [Primcodable β] [Inhabited β]
 
 variable {γ : Type w} [Primcodable γ] [Inhabited γ]
 
+#print toNat /-
 /-- Computable and injective mapping of predicates to sets of natural numbers.
 -/
 def toNat (p : Set α) : Set ℕ :=
   { n | p ((Encodable.decode α n).getD default) }
 #align to_nat toNat
+-/
 
+#print toNat_manyOneReducible /-
 @[simp]
 theorem toNat_manyOneReducible {p : Set α} : toNat p ≤₀ p :=
   ⟨fun n => (Encodable.decode α n).getD default,
     Computable.option_getD Computable.decode (Computable.const _), fun _ => Iff.rfl⟩
 #align to_nat_many_one_reducible toNat_manyOneReducible
+-/
 
+#print manyOneReducible_toNat /-
 @[simp]
 theorem manyOneReducible_toNat {p : Set α} : p ≤₀ toNat p :=
   ⟨Encodable.encode, Computable.encode, by simp [toNat, setOf]⟩
 #align many_one_reducible_to_nat manyOneReducible_toNat
+-/
 
+#print manyOneReducible_toNat_toNat /-
 @[simp]
 theorem manyOneReducible_toNat_toNat {p : Set α} {q : Set β} : toNat p ≤₀ toNat q ↔ p ≤₀ q :=
   ⟨fun h => manyOneReducible_toNat.trans (h.trans toNat_manyOneReducible), fun h =>
     toNat_manyOneReducible.trans (h.trans manyOneReducible_toNat)⟩
 #align many_one_reducible_to_nat_to_nat manyOneReducible_toNat_toNat
+-/
 
+#print toNat_manyOneEquiv /-
 @[simp]
 theorem toNat_manyOneEquiv {p : Set α} : ManyOneEquiv (toNat p) p := by simp [ManyOneEquiv]
 #align to_nat_many_one_equiv toNat_manyOneEquiv
+-/
 
+#print manyOneEquiv_toNat /-
 @[simp]
 theorem manyOneEquiv_toNat (p : Set α) (q : Set β) :
     ManyOneEquiv (toNat p) (toNat q) ↔ ManyOneEquiv p q := by simp [ManyOneEquiv]
 #align many_one_equiv_to_nat manyOneEquiv_toNat
+-/
 
+#print ManyOneDegree /-
 /-- A many-one degree is an equivalence class of sets up to many-one equivalence. -/
 def ManyOneDegree : Type :=
   Quotient (⟨ManyOneEquiv, equivalence_of_manyOneEquiv⟩ : Setoid (Set ℕ))
 #align many_one_degree ManyOneDegree
+-/
 
 namespace ManyOneDegree
 
+#print ManyOneDegree.of /-
 /-- The many-one degree of a set on a primcodable type. -/
 def of (p : α → Prop) : ManyOneDegree :=
   Quotient.mk'' (toNat p)
 #align many_one_degree.of ManyOneDegree.of
+-/
 
+#print ManyOneDegree.ind_on /-
 @[elab_as_elim]
 protected theorem ind_on {C : ManyOneDegree → Prop} (d : ManyOneDegree)
     (h : ∀ p : Set ℕ, C (of p)) : C d :=
   Quotient.inductionOn' d h
 #align many_one_degree.ind_on ManyOneDegree.ind_on
+-/
 
+#print ManyOneDegree.liftOn /-
 /-- Lifts a function on sets of natural numbers to many-one degrees.
 -/
 @[elab_as_elim, reducible]
@@ -385,13 +626,17 @@ protected def liftOn {φ} (d : ManyOneDegree) (f : Set ℕ → φ)
     (h : ∀ p q, ManyOneEquiv p q → f p = f q) : φ :=
   Quotient.liftOn' d f h
 #align many_one_degree.lift_on ManyOneDegree.liftOn
+-/
 
+#print ManyOneDegree.liftOn_eq /-
 @[simp]
 protected theorem liftOn_eq {φ} (p : Set ℕ) (f : Set ℕ → φ)
     (h : ∀ p q, ManyOneEquiv p q → f p = f q) : (of p).liftOn f h = f p :=
   rfl
 #align many_one_degree.lift_on_eq ManyOneDegree.liftOn_eq
+-/
 
+#print ManyOneDegree.liftOn₂ /-
 /-- Lifts a binary function on sets of natural numbers to many-one degrees.
 -/
 @[elab_as_elim, reducible, simp]
@@ -405,18 +650,23 @@ protected def liftOn₂ {φ} (d₁ d₂ : ManyOneDegree) (f : Set ℕ → Set �
       assumption
       rfl)
 #align many_one_degree.lift_on₂ ManyOneDegree.liftOn₂
+-/
 
+#print ManyOneDegree.liftOn₂_eq /-
 @[simp]
 protected theorem liftOn₂_eq {φ} (p q : Set ℕ) (f : Set ℕ → Set ℕ → φ)
     (h : ∀ p₁ p₂ q₁ q₂, ManyOneEquiv p₁ p₂ → ManyOneEquiv q₁ q₂ → f p₁ q₁ = f p₂ q₂) :
     (of p).liftOn₂ (of q) f h = f p q :=
   rfl
 #align many_one_degree.lift_on₂_eq ManyOneDegree.liftOn₂_eq
+-/
 
+#print ManyOneDegree.of_eq_of /-
 @[simp]
 theorem of_eq_of {p : α → Prop} {q : β → Prop} : of p = of q ↔ ManyOneEquiv p q := by
   simp [of, Quotient.eq'']
 #align many_one_degree.of_eq_of ManyOneDegree.of_eq_of
+-/
 
 instance : Inhabited ManyOneDegree :=
   ⟨of (∅ : Set ℕ)⟩
@@ -429,10 +679,12 @@ instance : LE ManyOneDegree :=
     ManyOneDegree.liftOn₂ d₁ d₂ (· ≤₀ ·) fun p₁ p₂ q₁ q₂ hp hq =>
       propext (hp.le_congr_left.trans hq.le_congr_right)⟩
 
+#print ManyOneDegree.of_le_of /-
 @[simp]
 theorem of_le_of {p : α → Prop} {q : β → Prop} : of p ≤ of q ↔ p ≤₀ q :=
   manyOneReducible_toNat_toNat
 #align many_one_degree.of_le_of ManyOneDegree.of_le_of
+-/
 
 private theorem le_refl (d : ManyOneDegree) : d ≤ d := by
   induction d using ManyOneDegree.ind_on <;> simp
@@ -473,6 +725,7 @@ instance : Add ManyOneDegree :=
             disjoin_manyOneReducible (hr₁.trans one_one_reducible.disjoin_left.to_many_one)
               (hr₂.trans one_one_reducible.disjoin_right.to_many_one)⟩)⟩
 
+#print ManyOneDegree.add_of /-
 @[simp]
 theorem add_of (p : Set α) (q : Set β) : of (p ⊕' q) = of p + of q :=
   of_eq_of.mpr
@@ -483,7 +736,9 @@ theorem add_of (p : Set α) (q : Set β) : of (p ⊕' q) = of p + of q :=
         (toNat_manyOneReducible.trans OneOneReducible.disjoin_left.to_many_one)
         (toNat_manyOneReducible.trans OneOneReducible.disjoin_right.to_many_one)⟩
 #align many_one_degree.add_of ManyOneDegree.add_of
+-/
 
+#print ManyOneDegree.add_le /-
 @[simp]
 protected theorem add_le {d₁ d₂ d₃ : ManyOneDegree} : d₁ + d₂ ≤ d₃ ↔ d₁ ≤ d₃ ∧ d₂ ≤ d₃ :=
   by
@@ -492,19 +747,24 @@ protected theorem add_le {d₁ d₂ d₃ : ManyOneDegree} : d₁ + d₂ ≤ d₃
   induction d₃ using ManyOneDegree.ind_on
   simpa only [← add_of, of_le_of] using disjoin_le
 #align many_one_degree.add_le ManyOneDegree.add_le
+-/
 
+#print ManyOneDegree.le_add_left /-
 @[simp]
 protected theorem le_add_left (d₁ d₂ : ManyOneDegree) : d₁ ≤ d₁ + d₂ :=
   (ManyOneDegree.add_le.1 (by rfl)).1
 #align many_one_degree.le_add_left ManyOneDegree.le_add_left
+-/
 
+#print ManyOneDegree.le_add_right /-
 @[simp]
 protected theorem le_add_right (d₁ d₂ : ManyOneDegree) : d₂ ≤ d₁ + d₂ :=
   (ManyOneDegree.add_le.1 (by rfl)).2
 #align many_one_degree.le_add_right ManyOneDegree.le_add_right
+-/
 
 instance : SemilatticeSup ManyOneDegree :=
-  { ManyOneDegree.partialOrder with
+  { ManyOneDegree.instPartialOrder with
     sup := (· + ·)
     le_sup_left := ManyOneDegree.le_add_left
     le_sup_right := ManyOneDegree.le_add_right
